Copello's combinator & Better alpha combinators

Lambda.v
@@ -1,4 +1,4 @@
-From Nominal Require Import Nominal Fresh.
+From Nominal Require Import Nominal Fresh Alpha NameAbstraction.
 From Nominal Require Import Instances.Name.
 
 Require Import FunInd.
@@ -60,9 +60,9 @@ Admitted.
 Inductive aeq: Term → Term → Prop :=
 | AeqVar: ∀ a, aeq (Var a) (Var a)
 | AeqApp: ∀ m n m' n', aeq m m' → aeq n n' → aeq (App m n) (App m' n')
-| AeqAbs: ∀ (a b: Name) (m n: Term), (∀ c,
-    (c <> a ∧ c <> b) → (c ∉ atm1 m ∧ c ∉ atm1 n) →
-    aeq (subst m c a) (subst n c b)) → aeq (Lam (a,m)) (Lam (b,n)).
+| AeqAbs: ∀ (a b: Name) (m n: Term), 
+    (∀ c, (c <> a ∧ c <> b) → (c ∉ atm1 m ∧ c ∉ atm1 n) → aeq (subst m c a) (subst n c b)) → 
+    aeq (Lam (a,m)) (Lam (b,n)).
 
 (* Necessario alguma relacao proper sobre os argumentos de aeq para
   facilitar reescrita *)
@@ -186,14 +186,6 @@ From Nominal Require Import Instances.SupportedFunctions
 Definition FCB `{Nominal X, Nominal Y} (f: X →ₛ Y) :=
   { a | a ∉ (support f) ∧ (∀ x: X, a # (f x)) }.
 
-(* Theorem freshness_theorem `{Nominal X} (f: Name →ₛ X): 
-  (∃ (c: Name), c ∉ support f ∧ c # (f c)) → 
-  ∀ a b, a # f → b # f → f a ≡ f b.
-Proof.
-
-They are both provable
-*)
-
 Theorem freshness_theorem `{Nominal X} (f: Name →ₛ X): 
   ∀ a b, (∃ (c: Name), c ∉ support f ∧ c # (f c)) → 
   a # f → b # f → f a ≡ f b.
@@ -211,8 +203,6 @@ Proof.
   - rewrite !fresh_fixpoint; try reflexivity; try assumption;
       apply fresh_fun_supp; auto; apply name_neq_fresh_iff, not_eq_sym; assumption.
 Qed.
-
-From Nominal Require Import Alpha NameAbstraction.
 
 Lemma perm_distr_1 (a b w z: Name) (p: Perm):
   w ≠ a → w ≠ b → z ≠ a → z ≠ b →
@@ -287,6 +277,12 @@ Proof. unfold action; simpl; reflexivity. Qed.
 Lemma action_app a b m n: ⟨a,b⟩ • App m n = App (⟨a,b⟩•m) (⟨a,b⟩•n).
 Proof. unfold action; simpl; reflexivity. Qed.
 
+Lemma perm_app p m n: p • App m n = App (p•m) (p•n).
+Admitted.
+
+Lemma perm_lam p a t: p • Lam (a, t) = Lam (p•a, p•t).
+Admitted.
+
 Lemma action_subst a b t: b ∉ atm1 t → (subst t b a) = ⟨a, b⟩ • t.
 Proof.
   intros; induction t using term_ind_general.
@@ -295,8 +291,6 @@ Proof.
   - simpl in *; rewrite action_app; f_equal; [apply IHt1 | apply IHt2]; set_solver.
   - simpl in *; rewrite action_lam; do 2 f_equal; [apply perm_swap_subst_name | apply IHt]; set_solver.
 Qed.
-
-Lemma perm_right_nil a b: ⟨a,b⟩ + nil ≡ ⟨a,b⟩. Proof. Admitted.
 
 Section AlphaStructural.
   Context `{Nominal X} (A: NameSet)
@@ -315,7 +309,7 @@ Section AlphaStructural.
       [apply Hd | |]; apply support_fresh; set_solver.
   Qed.
 
-  Definition supp_fvar (a: Name): Perm →ₛ X.
+  Definition g_var (a: Name): Perm →ₛ X.
     refine (λₛ⟦ support fvar ∪ support a ∪ A⟧ p : Perm, fvar (p • a)).
   Proof.
     - eabstract (intros ? ? HH; rewrite HH; reflexivity).
@@ -327,7 +321,7 @@ Section AlphaStructural.
           try (apply support_fresh; assumption); reflexivity).
   Defined.
 
-  Definition supp_fapp (Fm Fn: Perm →ₛ X): Perm →ₛ X.
+  Definition g_app (Fm Fn: Perm →ₛ X): Perm →ₛ X.
     refine (λₛ⟦ support fapp ∪ support Fm ∪ support Fn ∪ A⟧ p, fapp (Fm p, Fn p)).
   Proof.
     - eabstract (intros ? ? HH; rewrite HH; reflexivity).
@@ -338,19 +332,19 @@ Section AlphaStructural.
       rewrite fresh_fixpoint; try (apply support_fresh; assumption); reflexivity).
   Defined.
 
-  Definition supp_flam (a: Name) (Fm: Perm →ₛ X): Perm →ₛ X.
+  Definition g_lam (a: Name) (m: Term) (Fm: Perm →ₛ X): Perm →ₛ X.
     refine (
       λₛ⟦ support flam ∪ support a ∪ support (Fm) ∪ A ⟧ p,
-        let h: Name →ₛ X := λₛ⟦support flam ∪ support a ∪ support (Fm) ∪ support p ∪ A ⟧ a', (flam [a'](Fm (⟨a,a'⟩ + p))) in
+        let h: Name →ₛ X := λₛ⟦support flam ∪ support a ∪ support m ∪ support (Fm) ∪ support p ∪ A ⟧ a', (flam [a'](Fm (⟨a,a'⟩ + p))) in
         h (fresh (support h))
     ).
     all: swap 1 2.
     - intros w z Hw Hz p; cbn zeta.
-      set (g := (λₛ⟦ support flam ∪ support a ∪ support (Fm) ∪ support (⟨ w, z ⟩ • p) ∪ A ⟧ a' : Name, flam [a'](Fm (⟨ a, a' ⟩ + (⟨ w, z ⟩ • p))))).
-      set (h := (λₛ⟦ support flam ∪ support a ∪ support (Fm) ∪ support p ∪ A ⟧ a' : Name, flam [a'](Fm (⟨ a, a' ⟩ + p)))).
-      destruct (exist_fresh (support flam ∪ support a ∪ support (Fm) ∪ support w ∪ support z ∪ support (⟨ w, z ⟩ • p) ∪ support p ∪ A)) as [b Hb].
+      set (g := (λₛ⟦ _ ⟧ a' : Name, flam [a'](Fm (⟨ a, a' ⟩ + (⟨ w, z ⟩ • p))))).
+      set (h := (λₛ⟦ _ ⟧ a' : Name, flam [a'](Fm (⟨ a, a' ⟩ + p)))).
+      destruct (exist_fresh (support flam ∪ support a ∪ support m ∪ support (Fm) ∪ support w ∪ support z ∪ support (⟨ w, z ⟩ • p) ∪ support p ∪ A)) as [b Hb].
       rewrite (freshness_theorem g (fresh (support g)) b), (freshness_theorem h (fresh (support h)) b);
-      try (apply fresh_support_fresh); try (apply support_fresh; subst h g; unfold support at 1; simpl; set_solver).
+      try (apply fresh_support_fresh); try (apply support_fresh; subst h g; unfold support at 1; simpl; split_union; repeat (apply not_elem_of_union; split; try eauto)).
       all: swap 1 2. all: swap 2 3; try (subst; simpl; apply ft_flam).
       + subst g h; simpl.
         assert (HH: flam [b](Fm (⟨a,b⟩+(⟨w,z⟩•p))) ≡ flam [b]((⟨w,z⟩•(Fm)) (⟨w,z⟩•⟨a,b⟩+p))). {
@@ -367,10 +361,9 @@ Section AlphaStructural.
       - intros x y Hxy; cbn zeta; set (a' := fresh _); set (b' := fresh _).
         set (g := (λₛ⟦ _ ⟧ _ : Name, flam [_](Fm (⟨ a, _ ⟩ + x)))).
         set (h := (λₛ⟦ _ ⟧ _' : Name, flam [_](Fm (⟨ a, _ ⟩ + y)))).
-        destruct (exist_fresh (support flam ∪ support a ∪ support (Fm) ∪ support x ∪ support y ∪ support a' ∪ support b' ∪ A)) as [c Hc];
-        repeat (apply not_elem_of_union in Hc as [Hc ?]);
+        destruct (exist_fresh (support flam ∪ support a ∪ support m ∪ support (Fm) ∪ support x ∪ support y ∪ support a' ∪ support b' ∪ A)) as [c Hc];
         rewrite (freshness_theorem g a' c), (freshness_theorem h b' c);
-        try (apply fresh_support_fresh); try (apply support_fresh; subst h g; unfold support at 1; simpl; set_solver);
+        try (apply fresh_support_fresh); try (apply support_fresh; subst h g; unfold support at 1; simpl; split_union; repeat (apply not_elem_of_union; split; try eauto));
         try (subst; simpl; apply ft_flam);
         simpl; apply fsupp_equiv, nabs_inv, fsupp_equiv, grp_op_proper; auto.
   Unshelve. 
@@ -383,42 +376,36 @@ Section AlphaStructural.
 
   Fixpoint perm_alpha_rec (t: Term) : (Perm →ₛ X) :=
     match t with
-    | Var a => supp_fvar a
-    | App m n => supp_fapp (perm_alpha_rec m) (perm_alpha_rec n)
-    | Lam am => let (a, m) := am in supp_flam a (perm_alpha_rec m)
+    | Var a => g_var a
+    | App m n => g_app (perm_alpha_rec m) (perm_alpha_rec n)
+    | Lam am => let (a, m) := am in g_lam a m (perm_alpha_rec m)
     end.
 
-  (* Lemma perm_alpha_rec_var (a: Name):
-    perm_alpha_rec (Var a) = supp_fvar a.
-  Proof. simpl; reflexivity. Qed.
-
   Lemma perm_alpha_rec_app (m n: Term):
-    perm_alpha_rec (App m n) = supp_fapp (perm_alpha_rec m) (perm_alpha_rec n).
+    perm_alpha_rec (App m n) = g_app (perm_alpha_rec m) (perm_alpha_rec n).
   Proof. simpl; reflexivity. Qed.
 
   Lemma perm_alpha_rec_lam a (m: Term):
-    perm_alpha_rec (Lam [a]m) = supp_flam a m (perm_alpha_rec m).
-  Proof. simpl; reflexivity. Qed. *)
+    perm_alpha_rec (Lam (a,m)) = g_lam a m (perm_alpha_rec m).
+  Proof. simpl; reflexivity. Qed.
 
   Lemma alpha_rec_perm (t: Term):
     ∀ (p q: Perm), perm_alpha_rec t (q + p) ≡ perm_alpha_rec (q • t) p.
   Proof. 
     induction t using term_ind_general; intros.
     - simpl; rewrite gact_compat; reflexivity.
-    - admit.
-    - admit.
   Admitted.
 
   Theorem perm_alpha_rec_respectfull (m n : Term) :
     aeq m n → perm_alpha_rec m ≡ perm_alpha_rec n.
   Proof.
     induction 1.
-    - simpl; unfold supp_fvar; reflexivity.
-    - simpl; unfold supp_fapp; unfold equiv, fun_supp_equiv; intro p; simpl.
+    - simpl; unfold g_var; reflexivity.
+    - simpl; unfold g_app; unfold equiv, fun_supp_equiv; intro p; simpl.
       rewrite IHaeq1, IHaeq2; reflexivity.
-    - simpl; unfold supp_flam, equiv, fun_supp_equiv; intros p; simpl.
-      set (s1 := support flam ∪ support a ∪ support (perm_alpha_rec m) ∪ support p ∪ A);
-      set (s2 := support flam ∪ support b ∪ support (perm_alpha_rec n) ∪ support p ∪ A).
+    - simpl; unfold g_lam, equiv, fun_supp_equiv; intros p; simpl.
+      set (s1 := support flam ∪ support a ∪ support m ∪ support (perm_alpha_rec m) ∪ support p ∪ A);
+      set (s2 := support flam ∪ support b ∪ support n ∪ support (perm_alpha_rec n) ∪ support p ∪ A).
       set (h1 := (λₛ⟦ s1 ⟧ a' : Name, flam [a'](perm_alpha_rec m (⟨ a, a' ⟩ + p))));
       set (h2 := (λₛ⟦ s2 ⟧ a' : Name, flam [a'](perm_alpha_rec n (⟨ b, a' ⟩ + p)))).
       assert (HH1: flam [fresh (support h1)](perm_alpha_rec m (⟨ a, fresh (support h1) ⟩ + p)) = h1 (fresh (support h1))).
@@ -440,7 +427,10 @@ Section AlphaStructural.
       + apply support_fresh; set_solver.
   Qed.
 
-  Definition alpha_rec (t: Term) := perm_alpha_rec t nil.
+  Instance: Proper (aeq ==> equiv) (perm_alpha_rec).
+  Proof. repeat intro; apply perm_alpha_rec_respectfull. assumption. Qed.
+
+  Definition alpha_rec (t: Term) := perm_alpha_rec t ɛ.
 
   Lemma alpha_rec_var a : 
     alpha_rec (Var a) = fvar a.
@@ -451,7 +441,7 @@ Section AlphaStructural.
   Proof. unfold alpha_rec; simpl; reflexivity. Qed.
 
   Lemma alpha_rec_lam a m:
-    let h := fresh (support flam ∪ support a ∪ support (perm_alpha_rec m) ∪ A) in
+    let h := fresh (support flam ∪ support a ∪ support m ∪ support (perm_alpha_rec m) ∪ A) in
     alpha_rec (Lam [a]m) ≡ flam [h](alpha_rec (⟨a,h⟩•m)).
   Proof.
     intros; unfold alpha_rec; simpl; unfold support at 1; simpl.
@@ -459,10 +449,229 @@ Section AlphaStructural.
     assert (HH: h = b). { subst h b; unfold support; simpl; apply fresh_proper; set_solver. } 
     apply fsupp_equiv, name_abstraction_inv; left; split.
     - auto. 
-    - rewrite HH; apply alpha_rec_perm.
+    - rewrite HH, alpha_rec_perm; reflexivity.
+  Qed.
+
+  (* Lemma support_alpha m: support (perm_alpha_rec m) ⊆ support fvar ∪ support fapp ∪ support flam ∪ fv m.
+  Proof.
+    induction m using term_ind_general; simpl; unfold support at 1; admit.
+    Admitted.
+    (* - simpl. set_solver.
+    - set_solver.
+    - simpl. Search (_ ⊆ _ ∪ _). *) *)
+
+  (* Lemma alpha_rec_lam_exists m:
+    ∀ a, a ∉ (support fvar ∪ support fapp ∪ support flam) → 
+    alpha_rec (Lam [a]m) ≡ flam [a](alpha_rec m).
+  Proof.
+    intros; unfold alpha_rec; simpl; unfold support at 1; simpl.
+    set (w := fresh _).
+    apply fsupp_equiv, name_abstraction_inv; right; split.
+    - apply alpha_class_inv; right; split.
+      + apply not_eq_sym; apply name_neq_fresh_iff, support_fresh; subst w.
+        eapply not_elem_of_weaken.
+        * eapply is_fresh.
+        * set_solver.
+      + apply fresh_fun_supp; apply support_fresh; subst w; eapply not_elem_of_weaken;
+        try eapply is_fresh; set_solver.
+    - rewrite alpha_rec_perm, fun_equivar, (fresh_fixpoint w a).
+      + rewrite (fresh_fixpoint a w).
+        * apply fsupp_equiv; unfold action, perm_action.
+          rewrite grp_left_id, grp_left_inv; reflexivity.
+        * apply support_fresh; set_solver.
+        * apply support_fresh; subst w.
+          eapply not_elem_of_weaken.
+          -- eapply is_fresh.
+          -- set_solver.
+      + apply support_fresh; subst w; eapply not_elem_of_weaken.
+        * eapply is_fresh.
+        * set_solver.
+      + eapply support_fresh, not_elem_of_weaken.
+        * eauto.
+        * apply support_alpha.
+  Qed. *)
+
+  Lemma alpha_rec_lam_exists_abs m:
+    ∃ L: NameSet, ∀ a, a ∉ L → alpha_rec (Lam (a,m)) ≡ flam [a](alpha_rec m).
+  Proof.
+    exists (support flam ∪ support m ∪ support (perm_alpha_rec m)); intros.
+    intros; unfold alpha_rec; simpl; unfold support at 1; simpl.
+    set (w := fresh _).
+    apply fsupp_equiv, name_abstraction_inv; right; split.
+    - apply alpha_class_inv; right; split.
+      + apply not_eq_sym; apply name_neq_fresh_iff, support_fresh; subst w.
+        eapply not_elem_of_weaken.
+        * eapply is_fresh.
+        * set_solver.
+      + apply fresh_fun_supp; apply support_fresh; subst w; eapply not_elem_of_weaken;
+        try eapply is_fresh; set_solver.
+    - rewrite alpha_rec_perm, fun_equivar, (fresh_fixpoint w a).
+      + rewrite (fresh_fixpoint a w).
+        * apply fsupp_equiv; unfold action, perm_action.
+          rewrite grp_left_id, grp_left_inv; reflexivity.
+        * apply support_fresh; set_solver.
+        * apply support_fresh. subst w;
+          eapply not_elem_of_weaken.
+          -- eapply is_fresh.
+          -- set_solver.
+      + apply support_fresh; subst w; eapply not_elem_of_weaken.
+        * eapply is_fresh.
+        * set_solver.
+      + apply support_fresh; set_solver.
   Qed.
 
   Lemma alpha_rec_respectfull m n : 
     aeq m n → alpha_rec m ≡ alpha_rec n.
   Proof. intros; unfold alpha_rec; apply perm_alpha_rec_respectfull; assumption. Qed.
 End AlphaStructural.
+
+Lemma var_perm a p: p • (Var a) = Var (p • a).
+Proof. auto. Qed.
+
+Lemma app_perm m n p: p • (App m n) = App (p • m) (p • n).
+Proof. auto. Qed.
+
+Lemma lam_perm a m p: p • (Lam (a,m)) = Lam (p • a, p • m).
+Proof. auto. Qed.
+
+Lemma empty_perm (t: Term): ɛ • t = t.
+Proof. Admitted.
+
+
+(* Copello *)
+Definition term_rect_perm_general (P : Term → Type)
+  (fvar : ∀ a p, P (p • (Var a)))
+  (fapp : ∀ m, (∀ p, P (p • m)) → ∀ n, (∀ p, P (p • n)) → (∀ p, P (p • App m n)))
+  (flam : ∀ a m, (∀ p, P (p • m)) → (∀ p, P (p • (Lam (a,m))))): 
+  ∀ t p, P (p • t).
+Proof. 
+  induction t using term_rect_general; intros.
+  - intros; apply fvar.
+  - eapply fapp; eauto.
+  - eapply flam; eapply IHt.
+Qed.
+
+Class αCompat `{Equiv X} (P: X → Prop) := {
+  compat: ∀ m n, m ≡ n → P m → P n
+}.
+
+#[export] Instance αCompatProper `{αCompat X P}: Proper (equiv ==> impl) P.
+Proof. intros ? ? HH ?; eapply compat; eauto. Qed.
+
+#[export] Instance αCompatProperFlip `{αCompat X P}: Proper (equiv ==> flip impl) P.
+Proof. intros ? ? HH ?; eapply compat; eauto. Admitted.
+
+Lemma lam_abs_equiv (am bn: [𝔸]Term): am ≡ bn → Lam am ≡ Lam bn.
+Proof. Admitted. 
+
+Lemma alpha_ind_lam_aux:
+  ∀ P: Term → Prop, αCompat P →
+    ∀ L: NameSet, (∀ b m, b ∉ L → (∀ p, P (p • m)) → P (Lam [b]m)) →
+      ∀ a m, (∀ p, P (p • m)) → P (Lam [a]m).
+Proof.
+  intros ? ? L HL a m ?.
+  destruct (exist_fresh (support (Lam [a]m) ∪ support a ∪ L)) as
+    [z [[HLam ?]%not_elem_of_union ?]%not_elem_of_union].
+  apply compat with (Lam [z](⟨a,z⟩•m)).
+  - symmetry; apply lam_abs_equiv, name_abstraction_rename, support_fresh;
+      unfold support in HLam; simpl in *; apply not_elem_of_difference in HLam as [];
+      [assumption | set_solver].
+  - apply HL; [assumption |]; intros; rewrite gact_compat; auto.
+Qed.
+
+Definition alpha_ind:
+  ∀ P : Term → Prop, αCompat P →
+    (∀ a, P (Var a)) →
+    (∀ m n, P m → P n → P (App m n)) →
+    {L: NameSet | ∀ a m, a ∉ L → P m → P (Lam [a]m)} →
+  ∀ t, P t.
+Proof.
+  intros P αP Hvar Happ [L Habs] t; rewrite <-gact_id; apply term_rect_perm_general.
+  - intros; rewrite var_perm; apply Hvar.
+  - intros; rewrite app_perm; auto.
+  - intros; rewrite lam_perm; apply (alpha_ind_lam_aux _ αP) with L; intros.
+    + apply Habs; [| rewrite <-gact_id]; auto.  
+    + rewrite gact_compat; apply H.
+Qed.
+
+Section TermLength.
+
+  From Nominal Require Import Instances.Nat.
+  
+  Fixpoint term_length (t: Term): nat :=
+    match t with
+    | Var a => 1
+    | App m n => (term_length m) + (term_length n)
+    | Lam (a,m) => 1 + (term_length m)
+    end.
+
+  Definition length_fvar: Name →ₛ nat.
+  Proof. refine (λₛ⟦∅⟧ n, 1); intros; apply perm_nat. Defined.
+
+  Definition length_fapp: (nat * nat) →ₛ nat.
+  Proof. 
+    refine (λₛ⟦∅⟧ mn, ((fst mn) + (snd mn))%nat).
+    - intros [] [] [H1 H2]; simpl in *; rewrite H1,H2; reflexivity.
+    - intros ? ? ? ? []; simpl; rewrite !perm_nat; reflexivity.
+  Defined.
+
+  (* Instance: Reflexive (≈α). Proof. Admitted. *)
+  Instance: Proper (equiv ==> (≈α)) abs.
+  Proof. repeat intro; unfold equiv,name_abstraction_equiv in *;
+    destruct x as [[x n]]; destruct y as [[y m]]; assumption.
+  Qed.
+
+  Instance:  Proper (equiv ==> equiv) snd.
+  Proof. intros [] [] [? []]; simpl; rewrite !perm_nat in *; assumption. Qed.
+
+  Definition length_flam: [𝔸]nat →ₛ nat.
+  Proof.
+    refine (λₛ⟦∅⟧ (an: [𝔸]nat), (1 + (snd an))%nat).
+    - repeat intro. rewrite H; reflexivity.
+    - intros; rewrite !perm_nat; unfold action, name_abstraction_action; simpl; rewrite !perm_nat;
+      reflexivity.
+  Defined.
+
+  Lemma name_fresh_nat (a: Name) (n: nat): a # n. Proof. Admitted.
+
+  Lemma length_flam_fcb: FCB length_flam.
+  Proof.
+    unfold FCB; eexists; split.
+    - unfold support; simpl; apply not_elem_of_empty.
+    - intros; apply name_fresh_nat.
+  Unshelve.
+    (* we can use any name. Pick some default *)
+    exact Atom.default.
+  Qed.
+
+  Lemma term_lenght_respectfull: ∀ m n, m ≡ n → term_length m = term_length n.
+  Proof. Admitted.
+
+  (* Lemma length_equal:
+    ∀ t, term_length t = alpha_rec length_fvar length_fapp length_flam (lamFCB := length_flam_fcb) t.
+  Proof.
+    apply alpha_ind.
+    - apply Build_αCompat; intros; inversion H; subst;
+      erewrite alpha_rec_respectfull, term_lenght_respectfull; eauto; symmetry.
+      + assumption.
+      + constructor; assumption.
+    - intros; rewrite alpha_rec_var; simpl; reflexivity.
+    - intros ? ? A B; rewrite alpha_rec_app; simpl in *; rewrite A, B; reflexivity.
+    - eexists. intros. pose proof alpha_rec_lam_exists.
+      + simpl; auto.
+      + eapply H.   
+    
+    exists ∅. intros. rewrite alpha_rec_lam. set (w := fresh _). simpl in *.
+    
+    destruct (alpha_rec_lam_exists ∅ length_fvar length_fapp length_flam (lamFCB := length_flam_fcb) m).
+      rewrite H1. 
+
+
+
+    - rewrite alpha_rec_app, <-IHt1, <-IHt2; simpl; reflexivity.
+    - pose proof (alpha_rec_lam_exists_abs ∅ length_fvar length_fapp length_flam (lamFCB := length_flam_fcb)) t.
+      destruct H as [L ?].  rewrite H.
+      + simpl; rewrite IHt; reflexivity.
+      +  *)
+
+End TermLength.
