theories/Instances/Nat.v
@@ -1,0 +1,21 @@
+From Nominal Require Import Name Nominal Fresh.
+
+#[export] Instance nat_action: PermAction nat := fun p n => n.
+#[export] Instance nat_equiv: Equiv nat := eq.
+#[export] Instance nat_support: Support nat := fun n => ∅.
+
+#[export] Instance nat_perm: PermT nat.
+Proof. 
+    split; unfold equiv,nat_equiv,action,nat_action in *; repeat intro; auto.
+    - typeclasses eauto.
+Qed.
+
+#[export] Instance nat_nominal: Nominal nat.
+Proof. 
+    split; intros.
+    - apply nat_perm.
+    - reflexivity.
+Qed.
+
+Lemma perm_nat: ∀ (p: Perm) (n: nat), p • n = n.
+Proof. unfold action, nat_action; auto. Qed.
